theories/L/Complexity/Problems/TMGenNP_fixed_mTM.v
@@ -6,6 +6,8 @@ From Undecidability.L Require Import Tactics.LTactics Functions.Decoding TMflatF
 From Undecidability Require Import L.Functions.EqBool.
 From Undecidability Require Import L.Datatypes.LNat.
 
+(** For each Machine M (with n+1 tapes), we define this problem:
+Given n tapes and a sizeBound and a step bound, does there exist a (small enough) first tape such that the machine halts on the resulting n+1 tapes in fewer? *)
 
 Definition TMGenNP_fixed_mTM' (sig : finType) `{registered sig} n (M : mTM sig (S n)) : Vector.t (tape sig) n * nat * nat -> Prop :=
   fun '(ts, maxSize, steps) =>
@@ -15,6 +17,9 @@ Definition HaltsOrDiverges_fixed_mTM (sig : finType) `{registered sig} n (M : mT
   fun '(ts, maxSize, steps) =>
     forall t1, sizeOfTape t1 <= maxSize -> forall k f, loopM (initc M (t1:::ts)) steps = Some f -> k <= steps.
 
-Definition GenNPHalt_fixed_mTM (sig : finType) `{registered sig} n (M : mTM sig (S n))
+Definition TMGenNP_fixed_mTM (sig : finType) `{registered sig} n (M : mTM sig (S n))
   := restrictBy (HaltsOrDiverges_fixed_mTM M) (TMGenNP_fixed_mTM' M).
+
+Arguments TMGenNP_fixed_mTM : clear implicits.
+Arguments TMGenNP_fixed_mTM {_ _ _}.
 
