theories/L/Complexity/Reductions/TMGenNP/LM_to_mTM.v
@@ -1,0 +1,19 @@
+From Undecidability.L Require Import Tactics.LTactics.
+From Undecidability.L.Datatypes Require Import Lists LVector.
+From Undecidability.L.Complexity Require Import NP Synthetic Monotonic.
+From Undecidability.TM Require Import TM.
+
+
+From Undecidability.L.Complexity  Require Import LMGenNP TMGenNP_fixed_mTM.
+From Undecidability.L.AbstractMachines Require Import FlatPro.Computable.LPro.
+
+(* TODO: find: *)
+Axiom (sig:finType) (n:nat) (X:Type).
+Context `{R__sig : registered sig} `{registered X}.
+Axiom  (M : mTM sig (S n)) .
+
+Lemma LMGenNP_to_TMGenNP_mTM : LMGenNP X ⪯p TMGenNP_fixed_mTM M.
+Abort.
+
+
+
