theories/L/Complexity/Reductions/TMGenNP/L_to_LM.v
@@ -1,40 +1,16 @@
 From Undecidability.L Require Import Tactics.LTactics Prelim.MoreList Prelim.MoreBase.
-From Undecidability.L.Complexity Require Import NP Synthetic Monotonic GenNPHalt.
+From Undecidability.L.Complexity Require Import NP Synthetic Monotonic GenNP LMGenNP.
 
 From Undecidability.L Require Import LM_heap_def LM_heap_correct LBool ResourceMeasures Compile LNat LTerm Compile.
 
-(** The halting formulation of the generic NP-complete problem for the abstract machine executing L-terms. 
-This is usefull as we have a Turing machine that simulates this abstract machine. *)
-
-Definition initLMGen s c : (list (nat*list Tok)*list (nat*list Tok)*list (option ((nat * list Tok) * nat)))
-  := ([(0,s++c++[appT])],[],[]).
-
-Section fixX.
-  Context (X:Type) `{R__X : registered X}.
-  
-  Definition LMGenNPHalt' : list Tok*nat*nat -> Prop :=
-    fun '(P, maxSize, k (*in unary*)) =>
-      exists (c:X), size (enc c) <= maxSize /\ (exists sigma' k', k' <= k /\ evaluatesIn step k' (initLMGen P (compile (enc c))) sigma').
-
-  Definition LMHaltsOrDiverges : list Tok*nat*nat -> Prop :=
-    fun '(P, maxSize, steps (*in unary*)) =>
-      (exists s, P = compile s /\ proc s)
-      /\ forall (c : X), size (enc c) <= maxSize -> forall k sigma', evaluatesIn step k (initLMGen P (compile (enc c))) sigma' -> k <= steps.
-
-  Definition LMGenNPHalt := restrictBy LMHaltsOrDiverges LMGenNPHalt'.
-End fixX.
-
-Arguments LMGenNPHalt : clear implicits.
-Arguments LMGenNPHalt _ {_}.
-
-Lemma polyRed_GenNPHalt_to_LMGenNPHalt (X:Type) `{R__X : registered X}:
-  GenNPHalt X ⪯p LMGenNPHalt X.
+Lemma GenNP_to_LMGenNP (X:Type) `{R__X : registered X}:
+  GenNP X ⪯p LMGenNP X.
 Proof.
   evar (f__steps : nat -> nat). [f__steps]:intros n0.
   pose (f := (fun '(s, maxSize, steps) => (compile s,maxSize : nat, f__steps steps))).
   eapply reducesPolyMO_intro_restrictBy with (f:=f).
   2:{
-    intros [[s' maxSize] steps]. cbn - [GenNPHalt' LMGenNPHalt'].
+    intros [[s' maxSize] steps]. cbn - [GenNP' LMGenNP'].
     intros (cs&Hsize). assert (lambda s') as [s0 eq] by Lproc. set (s:=lam s0) in *. subst s'.
     split.
     -split. easy.
@@ -83,8 +59,8 @@ Proof.
   }
 Qed.
 
-Lemma NPhard_LMGenNPHalt X__cert `{R__cert : registered X__cert}:
-  canEnumTerms X__cert->  NPhard (LMGenNPHalt X__cert).
+Lemma NPhard_LMGenNP X__cert `{R__cert : registered X__cert}:
+  canEnumTerms X__cert->  NPhard (LMGenNP X__cert).
 Proof.
-  intros ?%NPhard_GenNPHalt. now eapply (red_NPhard polyRed_GenNPHalt_to_LMGenNPHalt).
+  intros ?%NPhard_GenNP. now eapply (red_NPhard GenNP_to_LMGenNP).
 Qed.
